lib/fdep.ml
@@ -1,1 +1,7 @@
+module State = Lang.Quint_State
 module Ex = Lang.Quint_Ex_TicTacToe
+
+let trace_tic_tac_toe ?(seed=0) ?(steps=10) () =
+  let steps = Prims.of_int steps in
+  let seed = Prims.of_int seed in
+  Ex.debug_trace steps seed
