tryf/Quint.State.fst
@@ -7,11 +7,13 @@ open FStar.List.Tot
 open Quint.Util
 open Quint.Ordered
 open Quint.Rng.Ops
+open Quint.Show
 
 module DM = FStar.DependentMap
 module List = FStar.List.Tot
 module Rng = Quint.Rng
 module Set = Quint.Set
+
 
 /// # State
 
@@ -19,68 +21,138 @@ module Set = Quint.Set
 ///
 /// Defines a state space
 class sig = {
-   /// `vars` is the set of "flexible variables"
-   vars:eqtype;
+   /// `var_t` is the set of "flexible variables"
+   var_t:eqtype;
+   /// Show a variable
+   show_var: var_t -> string;
+   /// `vars` is a list of all the variables
+   vars: list var_t;
    /// `types` maps each variable to the types of the values it can be assigned
-   types: vars -> Type
+   types: var_t -> Type;
 }
 
-let optional #k : (k -> Type) -> k -> Type =
+// TODO Contrib upstream
+(** If an element can be [index]ed, then it is a [mem] of the list. *)
+private
+let rec lemma_index_mem (#t:eqtype) (l:list t) (i:nat{i < length l}) :
+  Lemma
+    (ensures (index l i `mem` l))
+    [SMTPat (index l i `mem` l)]
+    =
+  match i with
+  | 0 -> ()
+  | _ -> lemma_index_mem (tl l) (i - 1)
+
+private
+let rec as_list_of_list_mems_aux (#a:eqtype) (l:list a) (i:nat{i < length l}) :
+  Tot (list (x:a{mem x l}))
+      (decreases length l - i)
+  =
+  if i = (length l - 1) then
+    [index l i]
+  else
+    index l i :: as_list_of_list_mems_aux l (i + 1)
+
+private
+let as_list_of_list_mems (#a:eqtype) (l:list a): list (x:a{mem x l}) =
+  match l with
+  | []   -> []
+  | _::_ -> as_list_of_list_mems_aux l 0
+
+private
+let _ex_as_list_of_list_mems =
+   let ls = ["a"; "b"; "c"] in
+   // let ls_t = x:string{List.mem x ls} in
+   let _ : list (x:string{List.mem x ls}) = as_list_of_list_mems ls in
+   ()
+
+let state_signature (vars : list string{length vars > 0}) (typef:(s:string{mem s vars} -> Type)) : sig =
+   let variables : list (x:string{List.mem x vars}) = as_list_of_list_mems #string vars in
+   { var_t = (x:string{mem x vars})
+   ; show_var = (fun s -> s)
+   ; vars  = variables
+   ; types = typef
+   }
+
+let optional #k : tf:(k -> Type) -> x:k -> t:Type{t == option (tf x)} =
   fun f v -> option (f v)
+
 
 // TODO Find a way to abstract implementation of this so we don't have to expose the
 // dep map impl.
 /// A state defined by a signature `sig`
-let state {| s:sig |} = DM.t vars (optional s.types)
+let state {| s:sig |} = DM.t var_t (optional s.types)
+
+// type concrete {|sig|} = list (v:var_t & types v)
 
 /// Predicates over states
 let is_assigned {| sig |} (m:state) k = Some? (DM.sel m k)
 let is_unassigned {| sig |} (m:state) k = None? (DM.sel m k)
-let is_fresh {| sig |} (m:state) = forall (v:vars). is_unassigned m v
-let is_updated {| sig |} (m:state) = forall (v:vars). is_assigned m v
+let is_fresh {| sig |} (m:state) = forall (v:var_t). is_unassigned m v
+let is_updated {| sig |} (m:state) = forall (v:var_t). is_assigned m v
 
-let init_opt {| sig |}: f:(v:vars -> types v) -> v':vars -> option (types v') =
+let as_concrete {|sg:sig|}
+  (s:(state #sg){is_updated #sg s})
+  : list (dtuple2 var_t types) =
+  List.map (fun v -> (| v, Some?.v (DM.sel s v) |)) sg.vars
+
+let init_opt {| sig |}: f:(v:var_t -> types v) -> v':var_t -> option (types v') =
   fun init variable -> Some (init variable)
 
 /// A state initialization function
-type init_t {|sig|} = v:vars -> types v
+type init_t {|sig|} = v:var_t -> types v
 
 /// Construct a state from an initialization function
 val init : sig -> init_t -> s:state{is_updated s}
 let init (s:sig) (f:init_t) : state = DM.create (init_opt f)
 
 let empty_state {| sig |} : m:state{is_fresh m} =
-  let clear _ = None in
+  let clear _  = None in
   DM.create (clear)
 
-let upd {| sig |} (v:vars) (x:types v)
+let upd {| sig |} (v:var_t) (x:types v)
   : m:state{is_unassigned m v} -> m':state{is_assigned m' v} =
   fun m -> DM.upd m v (Some x)
 
+
+
 // START State Example
 type ex_var = | V | U
-instance ex_sig : sig = {
-  vars = ex_var;
-  types = function
-    | V -> int
-    | U -> string
-}
+instance ex_sig : sig = state_signature
+  [ "v"; "u"]
+  (function
+  | "v" -> int
+  | "u" -> string)
+
 
 // Trying to update the same variable twice fails
-[@@expect_failure [54]]
-let _ex_cannot_update_twice = (~(upd V 1 empty_state |> upd V 10))
+[@@expect_failure [19]]
+let _ex_cannot_update_twice = (upd "v" 10 (upd "v" 1 empty_state))
 
-let _ex_is_updated_empty = assert_norm (~(is_updated (empty_state)))
-let _ex_is_updated_partial = assert_norm (~(is_updated (empty_state |> upd V 1)))
-let _ex_is_updated = assert_norm (is_updated ( upd V 1  empty_state |> upd U "foo" ))
+let _ex_is_updated = assert_norm (is_updated (upd "u" "foo" (upd "v" 1  empty_state)))
+
+let _ex_is_updated_empty = assert_norm (is_unassigned (empty_state ) "v")
+
+// let _ex_is_updated_partial = assert_norm (~(is_updated (upd "v" 1 empty_state )))
+
+
+
 
 let _s = init ex_sig (function
-  | V -> 0
-  | U -> "foo")
+  | "v" -> 0
+  | "u" -> "foo")
+
+let _ex_s_concrete = assert_norm (
+  as_concrete _s
+  =
+  [ (| "v", 0     |)
+  ; (| "u", "foo" |)
+  ]
+)
 
 let _ex_init = assert_norm (is_updated _s)
-let _ex_v = assert_norm (DM.sel _s V = Some 0)
-let _ex_x = assert_norm (DM.sel _s U = Some "foo")
+let _ex_v = assert_norm (DM.sel _s "v" = Some 0)
+let _ex_x = assert_norm (DM.sel _s "u" = Some "foo")
 // END State Example
 
 // TODO Use `DM.restrict` to limit map to just declared variables
@@ -105,24 +177,24 @@ let rec append_mem #t l1 l2 a = match l1 with
 // TODO Use `DM.restrict` to limit map to just declared variables
 // A computation of `a` that can read from `state #sig`
 // TODO Figure out how to hide and abstract these
-let state_has {|sig|} (s:state) (vs:list vars) =
+let state_has {|sig|} (s:state) (vs:list var_t) =
     forall v. mem v vs ==> is_assigned s v
 
-let state_not_has {|sig|} (s:state) (vs:list vars) =
+let state_not_has {|sig|} (s:state) (vs:list var_t) =
     forall v. mem v vs ==> is_unassigned s v
 
 let if_state_has_all_it_is_updated
     {|sig|}
     (s:state)
-    (vs:list vars)
-    : Lemma ((state_has s vs /\ (forall (v:vars). mem v vs)) ==> is_updated s)
+    (vs:list var_t)
+    : Lemma ((state_has s vs /\ (forall (v:var_t). mem v vs)) ==> is_updated s)
     // [SMTPat (state_has s vs); SMTPat (is_updated s)]
     = ()
 
 /// A computation of a value of type `a`,
 /// over a state defined by `sig`
 /// that can read from the variables in `list vars`
-type read {|sig|} (vs:list vars) (a:Type)
+type read {|sig|} (vs:list var_t) (a:Type)
   = s:state{state_has s vs} -> a
 
 let read_map {|sig|} #a #b #vs (f:a -> b) (x:read vs a) : read vs b
@@ -144,8 +216,8 @@ let pure {|sig|} #a #vs (x:a) : read vs a = fun _ -> x
 //   = fun s -> (x s, y s)
 
 /// Read a value of type `types v`
-val ( ! ) {| sig |} : v:vars -> read [v] (types v)
-let ( ! ) {| sig |} (v:vars) : read [v] (types v) // s:state{is_assigned s v} -> types v
+val ( ! ) {| sig |} : v:var_t -> read [v] (types v)
+let ( ! ) {| sig |} (v:var_t) : read [v] (types v) // s:state{is_assigned s v} -> types v
     =
     fun state -> Some?.v (DM.sel state v)
 
@@ -179,11 +251,11 @@ let (and!) {|sig|} #a #b #vs #vs'
   (x : read vs a) (y : read vs' b) : read (vs @ vs') (a * b)
   = fun s -> (x s, y s)
 
-let _read_ex : read [U; V] (int * string) =
-    let! x = !V
-    and! v = !U
+let _read_ex : read #ex_sig ["u"; "v"] (int * string) =
+    let! v = !"v"
+    and! u = !"u"
     in
-    (x, v)
+    (v, u)
 
 /// # State predicates: the *action* effect
 
@@ -195,7 +267,7 @@ let _read_ex : read [U; V] (int * string) =
 /// - `s0` is the current state
 /// - `s` is the intermediate state to be updated (lets us ensure no state is updated twice)
 /// - `s1` is the next state specified by by the action
-type action {|sig|} (vs:list vars)
+type action {|sig|} (vs:list var_t)
   = s0:state{is_updated s0}
     -> option (
       s:state{state_not_has s vs}
@@ -227,8 +299,8 @@ let ( !@ ) {|sig|} #rs #vs
     fun s0 -> ra s0 s0
 
 /// `v @= x` updates the state variable `v` to the value `x` in the next state
-val ( @= ) {|sig|} : v:vars -> x:types v -> action [v]
-let ( @= ) {|sig|} (v:vars) (x:types v) : action [v]
+val ( @= ) {|sig|} : v:var_t -> x:types v -> action [v]
+let ( @= ) {|sig|} (v:var_t) (x:types v) : action [v]
   = fun _ -> Some (fun s -> upd v x s)
 
 // TODO: replace ! with @ for consistency
@@ -299,12 +371,12 @@ module Set = Quint.Set
 /// # Transitions
 
 // A transition is an action that updates all the variables
-type transition {|sig|} #vs = a:action vs{(forall (v : vars). mem v vs)}
+type transition {|sig|} #vs = a:action vs{(forall (v : var_t). mem v vs)}
 
-let apply_det {|s:sig|} #vs
-  (t:transition #s #vs)
+let apply_det {|s:sig|}
+  (t:transition #s #vars)
   (s0:state{is_updated s0})
-  : option (s1:state{state_has s1 vs})
+  : option (s1:state{is_updated s1})
    =
   match t s0 with
   | None -> None
@@ -313,68 +385,147 @@ let apply_det {|s:sig|} #vs
 
 
 /// Apply a transition to the state
-let apply {|s:sig|} #vs
-  (nt:nondet (transition #s #vs))
+let apply {|s:sig|}
+  (nt:nondet (transition #s #vars))
   (s0:state{is_updated s0})
-  : nondet (option (s1:state{state_has s1 vs}))
+  : nondet (option (s1:state{is_updated s1}))
   =
   let? t = nt in
   apply_det t s0
 
-let rec run_aux {|s:sig|} #vs
-  (nt:nondet (transition #s #vs))
+module IO = FStar.IO
+
+let rec run_aux {|s:sig|}
+  (nt:nondet (transition #s #vars))
   (s0:state{is_updated s0})
-  : nat -> nondet (list state)
+  : c:nat
+  -> Tot (nondet (list (s1:state{is_updated s1})))
+         (decreases c)
   = function
-  | 0 -> return []
+  | 0 -> return [s0]
   | n ->
-  apply nt s0 >>= (function
-  | None    -> return []
-  | Some s1 ->
-  let? states = run_aux nt s0 (n - 1) in
-  s0 :: states)
+    let _ = IO.debug_print_string ("@ RUNNING STATE " ^ Prims.string_of_int n ^ "\n") in
+    apply nt s0 >>= (function
+  | None    ->
+    let _ = IO.debug_print_string ("@ DEADLOCK\n") in
+    // Report the last state run
+    return [s0]
+  | Some s1' ->
+    let _ = IO.debug_print_string ("@ STATE SUCEEDED\n") in
+    let? states = run_aux nt s1' (n - 1) in
+    s0 :: states)
 
 /// Run a transition for n_steps, or until it deadlocks
-let run {|s:sig|} #vs
+let run {|sg:sig|}
   (n_steps:nat)
   (i:init_t)
-  (nt:nondet (transition #s #vs)) =
-  let s0 = init s i in
+  (nt:nondet (transition #sg #vars))
+  (seed: nat)
+  : list (s:state{is_updated s})
+  =
+  let s0 = init sg i in
   run_aux nt s0 n_steps
+  |> Rng.run seed
 
-// TODO: need to adjust precedence so don't need to use brackets
-let _ex_conj_action : transition =
-  (  V @= 1
-  &@ U @= "foo"
-  )
+type trace_t {|sig|} = list (list (dtuple2 var_t types))
 
-let _ex_disj_action : action [V] =
-  (  V @= 1
-  |@ V @= 2
+let trace
+  {|sig|}
+  (states:list (s:state{is_updated s}))
+  : trace_t
+  =
+  List.map as_concrete states
+
+open Quint.Show
+open Quint.Map
+open Quint.Set
+
+let string_of_state_value
+  #a #b {|Show.show a|} {|Show.show b|}
+  (v:a) (u:b)
+  : string
+  =
+  to_string v ^ " -> " ^ to_string u
+
+
+// TODO: way to convert state values to string
+// let rec state_to_string
+//   {|sig|} (#v:var_t) {|show var_t|} {|show (types v)|}
+//   : (list (dtuple2 var_t types)) -> string
+//   = function
+//   | [] -> ""
+//   | (| a, b |) :: rest -> string_of_state_value a b ^ "\n" ^ state_to_string rest
+
+// let rec trace_to_string {|sig|} : trace_t -> string
+//   = function
+//   | [] -> ""
+//   | s :: ss -> state_to_string s ^ "\n---------\n" ^ trace_to_string ss
+
+// let run_debug {|sg:sig|}
+//   (n_steps:nat)
+//   (i:init_t)
+//   (nt:nondet (transition #sg #vars))
+//   (seed: nat)
+//   : string
+//   =
+//   trace_to_string (trace (run n_steps i nt seed))
+
+// instance show_trace {|sig|} : show (trace_t) = {
+//    to_string = trace_to_string
+// }
+
+let _ex_read_v : read ["v"] int =
+  let! v = !"v" in
+  v + 1
+
+let _ex_read_u : read ["u"] string =
+  let! u = !"u" in
+  u ^ "!"
+
+let _ex_composing_reads : read ["v"; "u"] (int * string) =
+  let! v' = _ex_read_v
+  and! u' = _ex_read_u
+  in
+  (v', u')
+
+let _ex_action_updating_v : action ["v"] =
+  "v" @= 1
+
+let _ex_action_updating_u : action ["u"] =
+ "u" @= "foo"
+
+let _ex_composing_actions : action ["v"; "u"]  =
+  _ex_action_updating_v
+  &@
+  _ex_action_updating_u
+
+let _ex_disj_action : action ["v"] =
+  (  "v" @= 1
+  |@ "v" @= 2
   )
 
 let _ex_comb_action : transition =
-  (  V @= 1
-  &@ U @= "foo"
+  (  "v" @= 1
+  &@ "u" @= "foo"
   )
   |@
-  (  V @= 10
-  &@ U @= "fee"
+  (  "v" @= 10
+  &@ "u" @= "fee"
   )
 
 
-let _ex_req_action : action [V; U] =
-  (  req (let! v = !V in v > 1)
-  &@ V @= 1
-  &@ U @= "foo"
+let _ex_req_action : action ["v"; "u"] =
+  (  req (let! v = !"v" in v > 1)
+  &@ "v" @= 1
+  &@ "u" @= "foo"
   ) |@ (  req (
-      let! v = !V
-      and! x = !U
+      let! v = !"v"
+      and! x = !"u"
       in
       v < 1 && x = "foo"
      )
-  &@ V @= 10
-  &@ U @= "fee"
+  &@ "v" @= 10
+  &@ "u" @= "fee"
   )
 
 let _ex_nondet_action : nondet transition
@@ -383,11 +534,11 @@ let _ex_nondet_action : nondet transition
     and? xr : string = one_of (Set.set["a"; "b"; "c"])
     in
     (  req (
-          let! v' = !V
-          and! x' = !U
+          let! v' = !"v"
+          and! x' = !"u"
           in
           v' > vr && x' = xr
        )
-    &@ V @= vr
-    &@ U @= xr
+    &@ "v" @= vr
+    &@ "u" @= xr
     )
