tryf/Quint.Show.fst
@@ -1,0 +1,49 @@
+module Quint.Show
+
+open FStar.Tactics.Typeclasses
+
+class show (a:Type) = {
+  to_string : a -> string
+}
+
+// instance show_fallback #a : show a = {
+//   to_string = fun _ -> "<opaque>"
+// }
+
+instance show_int : show int = {
+  to_string = Prims.string_of_int
+}
+
+instance show_string : show string = {
+  to_string = fun x -> "\"" ^ x ^ "\""
+}
+
+let rec list_to_string_aux #a (f : a -> string) : list a -> string = function
+ | [] -> "[]"
+ | [x] -> f x ^ " ]"
+ | x::xs -> f x ^ "; " ^ list_to_string_aux f xs
+
+let list_to_string #a (f : a -> string) (l:list a) : string =
+  "[ " ^ list_to_string_aux f l
+
+instance show_list #a {|show a|} : show (list a) = {
+  to_string = list_to_string to_string
+}
+
+instance show_pair #a #b {|show a|} {|show b|} : show (a * b) = {
+  to_string = fun (x, y) -> "(" ^ to_string x ^ ", " ^ to_string y ^ ")"
+}
+
+private
+let f #a {| show a |} (x:a) = to_string x
+
+private
+let _exv = [f 1; f "foo"; f [1;2;3]; f ("fii", 3)]
+
+private
+let _exs = assert_norm (
+  _exv
+  =
+
+  ["1"; "\"foo\""; "[ 1; 2; 3 ]"; "(\"fii\", 3)"]
+)
